theories/MaxOfTwoNumbers/Theorems/Attempt_02_SplitAttention.v
@@ -1,8 +1,8 @@
 From Coq Require Import Floats Sint63 Uint63 QArith Lia List PArray Derive.
 From NeuralNetInterp.Torch Require Import Tensor Einsum Slicing.
-From NeuralNetInterp.Util Require Import Pointed Wf_Uint63.
+From NeuralNetInterp.Util Require Import Pointed Wf_Uint63 Wf_Uint63.Instances SolveProperEqRel.
 From NeuralNetInterp.Util.Arith Require Import Classes Instances FloatArith.
-From NeuralNetInterp.Torch Require Import Tensor.Instances.
+From NeuralNetInterp.Torch Require Import Tensor.Instances Slicing.Instances.
 From NeuralNetInterp.TransformerLens Require Import HookedTransformer HookedTransformer.Instances.
 From NeuralNetInterp.MaxOfTwoNumbers Require Import Parameters Model Heuristics TheoremStatement Model.Instances.
 Import LoopNotation.
@@ -26,32 +26,253 @@ Local Ltac let_bind_hyp _ :=
 
 Local Ltac let_bind _ := repeat first [ progress cbv beta iota in * | let_bind_1 () | let_bind_hyp () ].
 
+Local Ltac let_bind_subst_shape _ :=
+  let_bind ();
+  repeat match goal with H : Shape _ |- _ => subst H end;
+  repeat match goal with H : forall b : bool, Shape _ |- _ => subst H end.
+
+#[export] Existing Instance reflexive_eq_dom_reflexive.
+#[local] Hint Constants Opaque : typeclass_instances.
+#[local] Typeclasses Transparent
+  relation fst snd
+  Classes.max Instances.Uint63.max has_default_max_leb
+  Classes.leb Instances.Uint63.leb
+  Classes.one
+  Shape ShapeType Shape.nil Shape.snoc Shape.app Shape.broadcast2 Shape.broadcast3 Shape.map Shape.map2 Shape.map3 Shape.hd Shape.tl Shape.ones Shape.repeat Shape.ShapeType.one
+  RawIndex RawIndexType RawIndex.nil RawIndex.snoc RawIndex.app RawIndex.hd RawIndex.tl
+  Index IndexType Index.nil Index.snoc Index.app Index.hd Index.tl
+  SliceIndex.transfer_shape SliceIndex.SliceIndexType.transfer_shape Slice.start Slice.stop Slice.step Slice.Concrete.length Slice.norm_concretize SliceIndex.SliceIndexType.transfer_shape_single_index
+  inject_int int_has_one
+  Rank Nat.radd
+  Classes.add Classes.div Classes.sub Classes.mul
+  has_add_with has_div_by has_sub_with has_mul_with
+  tensor tensor_of_rank
+  Tensor.eqfR
+  raw_get
+.
+#[export] Hint Transparent PrimInt63.leb : typeclass_instances.
+#[local] Set Keyed Unification.
+Local Ltac Proper_Tensor_eqf_t_step _
+  := match goal with
+     | [ |- Proper (_ ==> _) (fun x => _) ]
+       => intros ???
+     | [ |- Tensor.eqfR _ (fun x => _) (fun y => _) ]
+       => intro
+     | [ |- ?R (match ?x with _ => _ end) (match ?y with _ => _ end) ]
+       => tryif constr_eq x y
+         then destruct x eqn:?; subst
+         else destruct x eqn:?, y eqn:?; subst
+     | [ H : Tensor.eqfR _ ?x ?y |- _ ]
+       => move H at top;
+          first [ is_var x; revert dependent x; intros x H; setoid_rewrite H; clear H x; intros
+                | is_var y; revert dependent y; intros y H; setoid_rewrite <- H; clear H y; intros ]
+     | [ |- ?R ?x ?x ] => reflexivity
+     end.
+Local Ltac Proper_Tensor_eqf_t _ := repeat Proper_Tensor_eqf_t_step ().
+#[export] Hint Extern 1 (Proper (_ ==> _) (fun _ => _)) => progress Proper_Tensor_eqf_t () : typeclass_instances.
 Theorem good_accuracy : TheoremStatement.Accuracy.best (* (abs (real_accuracy - expected_accuracy) <? error)%float = true *).
 Proof.
   cbv [real_accuracy].
-  cbv beta iota delta [acc_fn]; let_bind ().
-  cbv beta iota delta [logits] in *; let_bind ().
-  repeat match goal with H : Shape _ |- _ => subst H end.
-  cbv beta iota delta [HookedTransformer.logits] in *; let_bind ().
-  repeat match goal with H : Shape _ |- _ => subst H end.
+  cbv beta iota delta [acc_fn]; let_bind_subst_shape ().
+  cbv beta iota delta [logits] in *; let_bind_subst_shape ().
+  cbv beta iota delta [HookedTransformer.logits] in *; let_bind_subst_shape ().
   cbv beta iota delta [blocks_params] in *.
-  cbv beta iota delta [HookedTransformer.blocks_cps fold_right HookedTransformer.blocks List.map] in *; let_bind ().
-  repeat match goal with H : Shape _ |- _ => subst H end.
+  cbv beta iota delta [HookedTransformer.blocks_cps fold_right HookedTransformer.blocks List.map] in *; let_bind_subst_shape ().
   vm_compute Shape.tl in *.
   vm_compute of_Z in *.
   vm_compute SliceIndex.transfer_shape in *.
   vm_compute Shape.app in *.
   vm_compute Shape.broadcast2 in *.
-  cbv beta iota delta [TransformerBlock.attn_only_out] in *; let_bind ().
-  subst maybe_n_heads.
-  cbv beta iota delta [Attention.attn_out] in *; let_bind ().
-  cbv beta iota delta [Attention.z] in *; let_bind ().
+  cbv beta iota delta [TransformerBlock.attn_only_out] in *; let_bind_subst_shape ().
+  cbv beta iota delta [Attention.attn_out] in *; let_bind_subst_shape ().
+  cbv beta iota delta [Attention.z] in *; let_bind_subst_shape ().
   set (v := Attention.v _ _ _) in *.
   set (pattern := Attention.pattern _ _ _ _ _ _) in *.
-  cbv beta iota delta [HookedTransformer.unembed] in *; let_bind ().
-  repeat match goal with H : Shape _ |- _ => subst H end.
-  cbv beta iota delta [Unembed.forward] in *; let_bind ().
-  repeat match goal with H : Shape _ |- _ => subst H end.
+  cbv beta iota delta [HookedTransformer.unembed] in *; let_bind_subst_shape ().
+  cbv beta iota delta [Unembed.forward] in *; let_bind_subst_shape ().
+  cbv beta iota delta [all_tokens] in true_maximum; let_bind_subst_shape ().
+  set (all_toks_c := PArray.checkpoint _) in (value of true_maximum).
+  set (out' := PArray.checkpoint _) in (value of out).
+  Local Ltac setoid_rewrite_in_body R lem H :=
+    let rewrite_or_error lem :=
+      let rew _ := (rewrite lem) (* first [ rewrite lem | setoid_rewrite lem ] *) in
+      tryif rew ()
+      then idtac
+      else (match goal with
+            | [ |- ?G ]
+              => let lemo := open_constr:(lem) in
+                 let T := type of lemo in
+                 idtac "Could not rewrite" lem ":" T "in goal" G
+            end;
+            rew ()) in
+    let ty := open_constr:(_) in
+    let H' := fresh H in
+    rename H into H';
+    evar (H : ty);
+    let lemH := fresh in
+    assert (lemH : R H' H) by (subst H'; rewrite_or_error lem; subst H; reflexivity);
+    let rec do_rewrite _
+      := lazymatch goal with
+         | [ H'' := context[H'] |- _ ]
+           => setoid_rewrite_in_body R lemH H'';
+              do_rewrite ()
+         | _ => idtac
+         end in
+    do_rewrite ();
+    lazymatch goal with
+    | [ |- context[H'] ] => rewrite_or_error lemH
+    | _ => idtac
+    end;
+    clear lemH; clear H'.
+  Tactic Notation "setoid_rewrite" "(" uconstr(R) ")" uconstr(lem) "in" "(" "value" "of" hyp(H) ")" := setoid_rewrite_in_body R lem H.
+  do 8 lazymatch goal with
+  | [ H := PArray.checkpoint _ |- _ ]
+    => setoid_rewrite (Tensor.eqf) Tensor.PArray.checkpoint_correct_eqf in (value of H)
+    end.
+  cbv beta iota delta [of_bool map map2] in res.
+  move true_maximum at bottom.
+  move all_toks_c at bottom.
+  move all_toks at bottom.
+  cbv beta iota delta [reduce_axis_m1 reduce_axis_m1' reshape_snoc_split RawIndex.curry_radd RawIndex.combine_radd map RawIndex] in true_maximum.
+  cbv beta iota delta [Reduction.max max has_default_max_leb leb] in true_maximum.
+  cbv -[PrimInt63.leb all_toks_c] in true_maximum.
+HERE
+  subst all_toks_c.
+  cbv beta iota delta [cartesian_prod] in true_maximum.
+  cbv beta iota delta [reshape_m1 modulo PrimInt63.mod Uint63.to_Z Uint63.to_Z_rec Uint63.size Uint63.is_even Uint63.is_zero Uint63.land Uint63.eqb Uint63.compare PrimInt63.lsr Z.double Z.succ_double Z.to_nat nth_default nth_error Pos.to_nat Pos.iter_op] in true_maximum.
+  cbv [raw_get] in true_maximum.
+  vm_compute PrimInt63.add in true_maximum.
+  cbv [tupleify] in true_maximum.
+  cbv [RawIndex.unreshape] in true_maximum.
+  cbv [RawIndex.unreshape'] in true_maximum.
+  cbv [RawIndex.item RawIndex.tl RawIndex.snoc RawIndex.nil fst snd Shape.hd RawIndex.hd Shape.tl Shape.snoc Shape.nil] in true_maximum.
+  move all_toks at bottom.
+  vm_compute of_Z in all_toks.
+  cbv [arange] in all_toks.
+  subst all_toks.
+  cbv [RawIndex.item RawIndex.tl raw_get] in true_maximum.
+  cbn [snd] in true_maximum.
+  cbn -[all_toks] in true_maximum'.
+  cbv [Uint63.to_Z Uint63.to_Z_red] in true_maximum'.
+
+  cbv [RawInde
+  cbv [
+  cbv [tupleify] in
+  cbn [
+  cbv -[all_toks] in true_maximum'.
+  subst true_maximum.
+  cbv
+  cbv
+
+
+  cbv beta iota delta [reduce_axis_m1 reduce_axis_m1' reshape_snoc_split RawIndex.curry_radd RawIndex.combine_radd map RawIndex] in pred_tokens.
+  Typeclasses eauto := debug.
+  #[export] Instance : Params (@Tensor.eqfR) 4 := {}.
+  #[export] Instance : Params (@Tensor.map2) 6 := {}.
+  #[export] Instance : Params (@Tensor.of_bool) 5 := {}.
+  #[export] Instance : Params (@SliceIndex.slice) 5 := {}.
+  #[export] Instance : Params (@map') 9 := {}.
+  try lazymatch goal with
+  | [ H := PArray.checkpoint _ |- _ ]
+    => setoid_rewrite (Tensor.eqf) Tensor.PArray.checkpoint_correct_eqf in (value of H)
+  end.
+  Unshelve.
+  2: { clear.
+       exact _.
+       generalize (@Tensor.map'_Proper_2).
+       generalize (@map'); intro map'.
+       repeat lazymatch goal with
+              | [ |- context[map' ?x] ]
+         => intro H; specialize (H x); revert H; generalize (map' x); clear map'; intro map'; assert_fails typeclasses eauto
+              end.
+       Set Typeclasses Debug Verbosity 2.
+       intro H.
+       try exact _.
+       intro H; specialize (H eq eq).
+
+       Set Typeclasses Debug.
+       try typeclasses eauto.
+       exact _.
+       Unshelve.
+       clear.
+       lazymatch goal with
+         | [ H : Tensor.eqfR _ ?x ?y |- _ ]
+           => move H at top;
+              is_var x;
+              revert dependent x; intros x H; setoid_rewrite H
+       end.
+              first [ is_var x; revert dependent x; intros x H; setoid_rewrite H; clear x; intros
+                    | is_var y; revert dependent y; intros y H; setoid_rewrite <- H; clear y; intros ]
+       end.
+       setoid_rewrite H.
+       reflexivity.
+       change (x ?i) with (raw_get x i).
+       change (y ?i) with (raw_get y i).
+       setoid_rewrite H.
+       Set Printing All.
+       intros ?? H.
+
+       Typeclasses eauto := debug.
+       Set Typeclasses Debug Verbosity 2.
+
+       try exact _.
+       assert ((@Shape.snoc
+                                                 (S (S O))
+                                                 (@Shape.snoc
+                                                    (S O)
+                                                    (@Shape.snoc O Shape.nil 0x1000)
+                                                    0x2) 0x40) =
+(@Shape.broadcast2 (S (S (S O)))
+   (@Shape.app (S (S O)) (S O)
+      (@Shape.snoc (S O) (@Shape.snoc O Shape.nil 0x1000) 0x2)
+      (@Shape.snoc O Shape.nil 0x40))
+   (@Shape.app (S (S O)) (S O) (@Shape.ones (S (S O)))
+      (@Shape.snoc O Shape.nil 0x40)))).
+       cbv [relation fst snd
+  Classes.max Instances.Uint63.max has_default_max_leb
+  Classes.leb Instances.Uint63.leb
+  Classes.one
+  Shape ShapeType Shape.nil Shape.snoc Shape.app Shape.broadcast2 Shape.broadcast3 Shape.map Shape.map2 Shape.map3 Shape.hd Shape.tl Shape.ones Shape.repeat Shape.ShapeType.one int_has_one
+  RawIndex RawIndexType RawIndex.nil RawIndex.snoc RawIndex.app RawIndex.hd RawIndex.tl
+  Index IndexType Index.nil Index.snoc Index.app Index.hd Index.tl
+  SliceIndex.transfer_shape SliceIndex.SliceIndexType.transfer_shape Slice.start Slice.stop Slice.step Slice.Concrete.length Slice.norm_concretize SliceIndex.SliceIndexType.transfer_shape_single_index
+  inject_int
+  Rank Nat.radd
+  Classes.add Classes.div Classes.sub Classes.mul
+  has_add_with has_div_by has_sub_with has_mul_with
+  tensor].
+       cbv [PrimInt63.leb].
+       cbv [one].
+      vm_compute.
+  2: { generalize (@Tensor.map'_Proper_2).
+       clear.
+       generalize (@map'); intro map'.
+       repeat lazymatch goal with
+       | [ |- context[map' ?x] ]
+         => intro H; specialize (H x); revert H; generalize (map' x); clear map'; intro map'; assert_fails typeclasses eauto
+              end.
+       intro H; specialize (H eq eq).
+       apply H.
+       exact _.
+       exact _.
+       exact _.
+       | [ H : context[Proper _ (?f
+       Set Printing Implicit.
+
+       (*Set Typeclasses Debug Verbosity 2.
+       Set Debug "tactic-unification".*)
+       try typeclasses eauto.
+
+  let ty := open_constr:(_) in
+  evar (res' : ty);
+  let lem := open_constr:(Tensor.eqf res res') in
+  unshelve erewrite (_ : lem);
+  [ subst res res'; rewrite Tensor.PArray.checkpoint_correct_eqf; reflexivity | clear res; rename res' into res ].
+  let res' := open_constr:(_) in
+  setoid_replace res with res'.
+  subst res.
+  rewrite
+  setoid_rewrite PArray.checkpoint_correct.
   cbv [item mean].
     cbv [reduce_axis_m1 reduce_axis_m1' reshape_snoc_split map RawIndex.curry_radd reshape_m1].
   cbv [raw_get].
