theories/Util/Wf_Uint63/Instances.v
@@ -95,39 +95,53 @@ Module Reduction.
     cbv [sum]; repeat intro.
     eapply map_reduce_Proper; repeat intro; cbv [pointwise_relation respectful] in *; subst; eauto.
   Qed.
+  #[export] Instance sum_Proper {A zeroA addA start stop step} : Proper (pointwise_relation _ eq ==> eq) (@sum A zeroA addA start stop step).
+  Proof. apply sum_Proper_pointwise. Qed.
   #[export] Instance prod_Proper_pointwise {A oneA mulA} : Proper (pointwise_relation _ (pointwise_relation _ (pointwise_relation _ (pointwise_relation _ eq ==> eq)))) (@prod A oneA mulA).
   Proof.
     cbv [prod]; repeat intro.
     eapply map_reduce_Proper; repeat intro; cbv [pointwise_relation respectful] in *; subst; eauto.
   Qed.
+  #[export] Instance prod_Proper {A oneA mulA start stop step} : Proper (pointwise_relation _ eq ==> eq) (@prod A oneA mulA start stop step).
+  Proof. apply prod_Proper_pointwise. Qed.
   #[export] Instance max_Proper_pointwise {A maxA} : Proper (pointwise_relation _ (pointwise_relation _ (pointwise_relation _ (pointwise_relation _ eq ==> eq)))) (@max A maxA).
   Proof.
     cbv [max]; repeat intro.
     eapply map_reduce_no_init_Proper; repeat intro; cbv [pointwise_relation respectful] in *; subst; eauto.
   Qed.
+  #[export] Instance max_Proper {A maxA start stop step} : Proper (pointwise_relation _ eq ==> eq) (@max A maxA start stop step).
+  Proof. apply max_Proper_pointwise. Qed.
   #[export] Instance min_Proper_pointwise {A minA} : Proper (pointwise_relation _ (pointwise_relation _ (pointwise_relation _ (pointwise_relation _ eq ==> eq)))) (@min A minA).
   Proof.
     cbv [min]; repeat intro.
     eapply map_reduce_no_init_Proper; repeat intro; cbv [pointwise_relation respectful] in *; subst; eauto.
   Qed.
+  #[export] Instance min_Proper {A minA start stop step} : Proper (pointwise_relation _ eq ==> eq) (@min A minA start stop step).
+  Proof. apply min_Proper_pointwise. Qed.
   #[export] Instance argmax_Proper_pointwise {A ltbA} : Proper (pointwise_relation _ (pointwise_relation _ (pointwise_relation _ (pointwise_relation _ eq ==> eq)))) (@argmax A ltbA).
   Proof.
     cbv [argmax]; repeat intro.
     erewrite map_reduce_no_init_Proper; try reflexivity.
     cbv in *; intros; congruence.
   Qed.
+  #[export] Instance argmax_Proper {A ltbA start stop step} : Proper (pointwise_relation _ eq ==> eq) (@argmax A ltbA start stop step).
+  Proof. apply argmax_Proper_pointwise. Qed.
   #[export] Instance argmin_Proper_pointwise {A lebA} : Proper (pointwise_relation _ (pointwise_relation _ (pointwise_relation _ (pointwise_relation _ eq ==> eq)))) (@argmin A lebA).
   Proof.
     cbv [argmin]; repeat intro.
     erewrite map_reduce_no_init_Proper; try reflexivity.
     cbv in *; intros; congruence.
   Qed.
+  #[export] Instance argmin_Proper {A lebA start stop step} : Proper (pointwise_relation _ eq ==> eq) (@argmin A lebA start stop step).
+  Proof. apply argmin_Proper_pointwise. Qed.
   #[export] Instance mean_Proper_pointwise {A B C zeroA addA div_byABC coerB} : Proper (pointwise_relation _ (pointwise_relation _ (pointwise_relation _ (pointwise_relation _ eq ==> eq)))) (@mean A B C zeroA addA div_byABC coerB).
   Proof.
     cbv [mean]; repeat intro.
     erewrite sum_Proper_pointwise by eassumption.
     reflexivity.
   Qed.
+  #[export] Instance mean_Proper {A B C zeroA addA div_byABC coerB start stop step} : Proper (pointwise_relation _ eq ==> eq) (@mean A B C zeroA addA div_byABC coerB start stop step).
+  Proof. apply mean_Proper_pointwise. Qed.
   #[export] Instance var_Proper_pointwise {A B zeroA addA mulA subA div_byAB coerB correction} : Proper (pointwise_relation _ (pointwise_relation _ (pointwise_relation _ (pointwise_relation _ eq ==> eq)))) (@var A B zeroA addA mulA subA div_byAB coerB correction).
   Proof.
     cbv [var]; repeat intro.
@@ -137,5 +151,7 @@ Module Reduction.
     cbv [pointwise_relation] in *.
     congruence.
   Qed.
+  #[export] Instance var_Proper {A B zeroA addA mulA subA div_byAB coerB correction start stop step} : Proper (pointwise_relation _ eq ==> eq) (@var A B zeroA addA mulA subA div_byAB coerB correction start stop step).
+  Proof. apply var_Proper_pointwise. Qed.
 End Reduction.
 Export (hints) Reduction.
